

Seminar 3

1. Rijndael Block Cipher

$$A = (73)_{16} = (\underset{2^2}{0} \underset{2^1}{1} \underset{2^0}{1} \underset{2^3}{0} \underset{2^2}{0} \underset{2^1}{1} \underset{2^0}{1})_2$$

$$= x^6 + x^5 + x^4 + x^1 + 1$$

$$B = (4E)_{16} = (0 \underset{2^3}{1} \underset{2^2}{0} \underset{2^1}{0} \underset{2^0}{0} \underset{2^3}{1} \underset{2^2}{1} \underset{2^1}{0})_2$$

$$= x^6 + x^3 + x^2 + x$$

$$C = (85)_{16} = (1 \underset{2^3}{0} \underset{2^2}{0} \underset{2^1}{0} \underset{2^0}{0} \underset{2^3}{0} \underset{2^2}{1} \underset{2^1}{0})_2 = x^2 + x^2 + 1$$

$$A + B = (x^6 + x^5 + x^4 + x + 1) + (x^6 + x^3 + x^2 + x) = x^5 + x^4 + x^3 + x^2 + 1$$

$$(A+B) \cdot C = \frac{(x^5 + x^4 + x^3 + x^2 + 1)(x^2 + x^2 + 1)}{(x^2 + x^2 + 1)}$$

$$\frac{x^{12} + x^{11} + x^{10} + x^9 + x^8 + x^7 + x^6 + x^5 + x^4 + x^3 + x^2 + x + 1}{x^2 + x^2 + 1}$$

$$(A+B) \cdot C = (x^5 + x^4 + x^3 + x^2 + 1)(x^2 + x^2 + 1) = x^{12} + x^{11} + x^{10} + x^9 + x^8 + x^7 + x^6 + x^5 + x^4 + x^3 + x^2 + x + 1$$

$$= x^{12} + x^{11} + x^{10} + x^9 + x^8 + x^7 + x^6 + x^5 + 1$$

$$G(x^8): (A+B) \cdot C \bmod (x^8 + x^4 + x^3 + x + 1)$$

$ \begin{array}{r} x^{12} + x^{11} + x^{10} + x^9 + x^8 + x^7 + x^6 + x^5 + 1 \\ \underline{x^{12} + x^8 + x^2 + x^5 + x^4} \\ x^{11} + x^{10} + x^9 + x^8 + x^7 + x^6 + x^5 + x^4 + 1 \\ \underline{x^{11} + x^2 + x^6 + x^4 + x^3} \\ x^{10} + x^9 + x^8 + x^7 + x^6 + x^5 + x^3 + 1 \\ \underline{x^{10} + x^6 + x^5 + x^3 + x^2} \\ x^9 + x^8 + x^7 + x^6 + x^5 + x^3 + 1 \\ \underline{x^9 + x^5 + x^4 + x^2 + x} \\ x^8 + x^6 + x^5 + x^4 + x^3 + x + 1 \\ \underline{x^8 + x^4 + x^3 + x + 1} \\ x^6 + x^5 \end{array} $	$ \begin{array}{r} x^8 + x^4 + x^3 + x + 1 \\ \underline{x^4 + x^3 + x^2 + x + 1} \\ x^8 + x^4 + x^3 + x + 1 \end{array} $
---	--